Thm.s encode_element2d_+{vc,cv,cc} done

examples/pseudo_bool/cp_encoding/cp_to_ilpScript.sml
@@ -1420,8 +1420,8 @@ Proof
   gvs[reify_tuple_eq_sem,GSYM MAP_LIST_REL]
 QED
 
-Theorem le_int_of_num_Num:
-  1 ≤ X ∧ X ≤ &Y ⇒ 1 ≤ Num X ∧ Num X ≤ Y
+Triviality numint_le:
+  (Num X ≤ Y ⇒ X ≤ &Y) ∧ (1 ≤ X ∧ X ≤ &Y ⇒ 1 ≤ Num X ∧ Num X ≤ Y)
 Proof
   intLib.ARITH_TAC
 QED
@@ -1429,19 +1429,16 @@ QED
 (* encode_element2d for constant X and variable Y *)
 Definition encode_element2d_cv_def:
   encode_element2d_cv bnd R X Y Tss =
-  if 1 ≤ X ∧ X ≤ &LENGTH Tss ∧ EVERY (λTs. LENGTH Ts = LENGTH $ HD Tss) Tss
+  if EVERY (λTs. LENGTH Ts = LENGTH $ HD Tss) Tss ∧ 1 ≤ X ∧ X ≤ &LENGTH Tss
   then encode_element_var bnd R Y $ EL (Num X - 1) Tss
   else [([],[],1)]
 End
 
 Theorem encode_element2d_cv_sem:
   valid_assignment bnd wi ⇒
-  EVERY (λx. iconstraint_sem x (wi,wb))
-    (encode_element2d_cv bnd R X Y Tss) = (
-  (∀i. 1 ≤ i ∧ i ≤ LENGTH (EL (Num X - 1) Tss) + 1 ⇒
-    (wb (Ge Y (&i)) ⇔ wi Y ≥ &i)) ∧
-  (∀i. 1 ≤ i ∧ i ≤ LENGTH (EL (Num X - 1) Tss) ⇒
-    (wb (Eq Y (&i)) ⇔ wi Y = &i)) ∧
+  EVERY (λx. iconstraint_sem x (wi,wb)) (encode_element2d_cv bnd R X Y Tss) = (
+  (∀j. 1 ≤ j ∧ j ≤ LENGTH (HD Tss) + 1 ⇒ (wb (Ge Y (&j)) ⇔ wi Y ≥ &j)) ∧
+  (∀j. 1 ≤ j ∧ j ≤ LENGTH (HD Tss) ⇒ (wb (Eq Y (&j)) ⇔ wi Y = &j)) ∧
   element2d_sem R (INR X) (INL Y) Tss wi)
 Proof
   strip_tac>>
@@ -1449,51 +1446,55 @@ Proof
   IF_CASES_TAC
   >-(
     fs[encode_element_var_sem,element_sem_def,varc_def,EVERY_EL]>>
-    ‘1 ≤ Num X ∧ Num X ≤ LENGTH Tss’ suffices_by simp[]>>
-    metis_tac[le_int_of_num_Num])>>
+    imp_res_tac numint_le>>
+    simp[])>>
   simp[iconstraint_sem_def,eval_lin_term_def,eval_ilin_term_def,iSUM_def,varc_def]>>
-  metis_tac[GSYM NOT_EVERY,intLib.ARITH_PROVE “Num X ≤ Y ⇒ X ≤ &Y”]
+  metis_tac[GSYM NOT_EVERY,numint_le]
 QED
 
 (* encode_element2d for variable X and constant Y *)
 Definition encode_element2d_vc_def:
   encode_element2d_vc bnd R X Y Tss =
-  if 0 < LENGTH Tss ∧ EVERY (λTs. LENGTH Ts = LENGTH $ HD Tss) Tss ∧
+  if EVERY (λTs. LENGTH Ts = LENGTH $ HD Tss) Tss ∧ 0 < LENGTH Tss ∧
     1 ≤ Y ∧ Y ≤ &(LENGTH $ HD Tss)
   then encode_element_var bnd R X $ MAP (EL (Num Y - 1)) Tss
   else [([],[],1)]
 End
 
+Theorem EL_LIST2D:
+  m < LENGTH ls ⇒ EL m (MAP (EL n) ls) = EL n (EL m ls)
+Proof
+  strip_tac>>
+  irule EL_MAP>>
+  simp[]
+QED
+
 Theorem encode_element2d_vc_sem:
   valid_assignment bnd wi ⇒
-  EVERY (λx. iconstraint_sem x (wi,wb))
-    (encode_element2d_vc bnd R X Y Tss) = (
-  0 < LENGTH Tss ∧
-  (∀i. 1 ≤ i ∧ i ≤ LENGTH (MAP (EL (Num Y - 1)) Tss) + 1 ⇒
-    (wb (Ge X (&i)) ⇔ wi X ≥ &i)) ∧
-  (∀i. 1 ≤ i ∧ i ≤ LENGTH (MAP (EL (Num Y - 1)) Tss) ⇒
-    (wb (Eq X (&i)) ⇔ wi X = &i)) ∧
+  EVERY (λx. iconstraint_sem x (wi,wb)) (encode_element2d_vc bnd R X Y Tss) = (
+  (∀i. 1 ≤ i ∧ i ≤ LENGTH Tss + 1 ⇒ (wb (Ge X (&i)) ⇔ wi X ≥ &i)) ∧
+  (∀i. 1 ≤ i ∧ i ≤ LENGTH Tss ⇒ (wb (Eq X (&i)) ⇔ wi X = &i)) ∧
   element2d_sem R (INL X) (INR Y) Tss wi)
 Proof
   strip_tac>>
   simp[encode_element2d_vc_def,element2d_sem_def]>>
   IF_CASES_TAC
   >-(
-    fs[encode_element_var_sem,element_sem_def,varc_def,EVERY_EL]>>
-    ‘EL (Num (wi X) − 1) (MAP (EL (Num Y − 1)) Tss) =
-      EL (Num Y − 1) (EL (Num (wi X) − 1) Tss)’ by cheat>>
-    pop_assum (fn thm => simp[thm])>>
-    ‘Num Y ≤ LENGTH (HD Tss)’ suffices_by simp[]>>
-    simp[le_int_of_num_Num])>>
-  simp[iconstraint_sem_def,eval_lin_term_def,eval_ilin_term_def,iSUM_def,varc_def]>>
-  fs[Once LENGTH_NON_NIL,Once $ GSYM NOT_EVERY]>>
-  ‘¬(Num Y ≤ LENGTH (HD Tss))’ suffices_by simp[]>>
-  intLib.ARITH_TAC
+    fs[encode_element_var_sem,element_sem_def,varc_def,EVERY_EL,numint_le,
+      CONJ_ASSOC]>>
+    match_mp_tac $ METIS_PROVE[] “(R ⇒ (P ⇔ Q)) ⇒
+      ((R' ∧ R) ∧ P ⇔ (R' ∧ R) ∧ Q)”>>
+    strip_tac>>
+    fs[EL_LIST2D])>>
+  fs[iconstraint_sem_def,eval_lin_term_def,eval_ilin_term_def,iSUM_def,varc_def,
+    Once LENGTH_NON_NIL,Once $ GSYM NOT_EVERY]>>
+  metis_tac[numint_le]
 QED
 
+(* encode_element2d for constant X and constant Y *)
 Definition encode_element2d_cc_def:
   encode_element2d_cc bnd R X Y Tss =
-  if 0 < LENGTH Tss ∧ EVERY (λTs. LENGTH Ts = LENGTH $ HD Tss) Tss ∧
+  if EVERY (λTs. LENGTH Ts = LENGTH $ HD Tss) Tss ∧
     1 ≤ X ∧ X ≤ &LENGTH Tss ∧ 1 ≤ Y ∧ Y ≤ &(LENGTH $ HD Tss)
   then [
     mk_constraint_ge 1 (EL (Num Y - 1) $ EL (Num X - 1) Tss) (-1) R 0;
@@ -1505,25 +1506,68 @@ Theorem encode_element2d_cc_sem:
   EVERY (λx. iconstraint_sem x (wi,wb)) (encode_element2d_cc bnd R X Y Tss) =
   element2d_sem R (INR X) (INR Y) Tss wi
 Proof
-  cheat
+  rw[encode_element2d_cc_def,mk_constraint_ge_sem,element2d_sem_def,eval_raw,
+    varc_def,numint_le]
+  >-intLib.ARITH_TAC>>
+  metis_tac[numint_le,GSYM NOT_EVERY]
 QED
 
-Definition encode_element2d_eq_def:
-  encode_element2d_eq bnd R X Y (i:num,j:num,Aij) = [
-    bits_imply bnd [Pos (Eq X (&(i + 1)));Pos (Eq Y (&(j + 1)))]
-      (mk_constraint_ge 1 Aij (-1) R 0);
-    bits_imply bnd [Pos (Eq X (&(i + 1)));Pos (Eq Y (&(j + 1)))]
-      (mk_constraint_ge 1 R (-1) Aij 0)]
-End
-
+(* encodes X ≥ 1,...,X ≥ n *)
 Definition encode_ges_def:
   encode_ges bnd X n = FLAT (GENLIST (λi. encode_ge bnd X (&(i + 1))) n)
 End
 
+Theorem encode_ges_sem:
+  valid_assignment bnd wi ⇒
+  EVERY (λx. iconstraint_sem x (wi,wb)) (encode_ges bnd X n) =
+  EVERY (λv. wb (Ge X v) ⇔ wi X ≥ v) $ GENLIST (λi. &(i + 1)) n
+Proof
+  rw[encode_ges_def,EVERY_FLAT,EVERY_GENLIST]>>
+  ho_match_mp_tac FORALL_IMP_EQ>>
+  rw[encode_ge_sem]
+QED
+
+(* encodes X = 1,...,X = n *)
 Definition encode_eqs_def:
   encode_eqs bnd X n = FLAT (GENLIST (λi. encode_eq bnd X (&(i + 1))) n)
 End
 
+Theorem encode_eqs_sem:
+  valid_assignment bnd wi ∧
+  EVERY (λv. wb (Ge X v) ⇔ wi X ≥ v) $ GENLIST (λi. &(i + 1)) (n + 1) ⇒
+  EVERY (λx. iconstraint_sem x (wi,wb)) (encode_eqs bnd X n) =
+  EVERY (λv. wb (Eq X v) ⇔ wi X = v) $ GENLIST (λi. &(i + 1)) n
+Proof
+  rw[encode_eqs_def,EVERY_FLAT,EVERY_GENLIST]>>
+  ho_match_mp_tac FORALL_IMP_EQ>>
+  rw[]>>
+  irule encode_eq_sem>>
+  last_x_assum (fn thm => simp[thm,GSYM integerTheory.INT])>>
+  pure_rewrite_tac[ADD1]>>
+  last_assum $ irule>>
+  intLib.ARITH_TAC
+QED
+
+Definition encode_element2d_eq_def:
+  encode_element2d_eq bnd R X Y (i:num,j:num,Aij) = [
+    bits_imply bnd [Pos (Eq X &(i + 1));Pos (Eq Y &(j + 1))]
+      (mk_constraint_ge 1 Aij (-1) R 0);
+    bits_imply bnd [Pos (Eq X &(i + 1));Pos (Eq Y &(j + 1))]
+      (mk_constraint_ge 1 R (-1) Aij 0)]
+End
+
+Theorem encode_element2d_eq_sem:
+  valid_assignment bnd wi ∧
+  (wb (Eq X &(i + 1)) ⇔ wi X = &(i + 1)) ∧
+  (wb (Eq Y &(j + 1)) ⇔ wi Y = &(j + 1)) ⇒
+  EVERY (λx. iconstraint_sem x (wi,wb)) (encode_element2d_eq bnd R X Y (i,j,Aij)) = (
+    wi X = &(i + 1) ∧ wi Y = &(j + 1) ⇒ varc wi R = varc wi Aij)
+Proof
+  rw[encode_element2d_eq_def,eval_raw,bits_imply_sem,mk_constraint_ge_sem]>>
+  intLib.ARITH_TAC
+QED
+
+(* encode_element2d for variable X and variable Y *)
 Definition encode_element2d_vv_def:
   encode_element2d_vv bnd R X Y Tss =
   let
@@ -1535,30 +1579,18 @@ Definition encode_element2d_vv_def:
         m = LENGTH $ HD Tss;
         (lbX,ubX) = bnd X;
         (lbY,ubY) = bnd Y;
-        gesX = encode_ges bnd X (n + 1);
-        gesY = encode_ges bnd Y (m + 1);
-        eqsX = encode_eqs bnd X n;
-        eqsY = encode_eqs bnd Y m;
         xlb = if lbX < 1 then [([(1i,X)],[],1i)] else [];
         xub = if &n < ubX then [([(-1i,X)],[],-&n)] else [];
         ylb = if lbY < 1 then [([(1i,Y)],[],1i)] else [];
         yub = if &m < ubY then [([(-1i,Y)],[],-&n)] else [];
         mat = enumerate 0 $ MAP (λTs. enumerate 0 Ts) Tss
       in
-        gesX ++ gesY ++ eqsX ++ eqsY ++
+        encode_ges bnd X (n + 1) ++ encode_ges bnd Y (m + 1) ++
+        encode_eqs bnd X n ++ encode_eqs bnd Y m ++
         xlb ++ xub ++ ylb ++ yub ++
         (FLAT $ MAP (λ(i,vec).
-           FLAT $ MAP (λp. encode_element2d_eq bnd R X Y (i,p)) vec) mat)
+          FLAT $ MAP (λp. encode_element2d_eq bnd R X Y (i,p)) vec) mat)
     else [([],[],1)]
-End
-
-Definition encode_element2d_def:
-  encode_element2d bnd R X Y Tss =
-  case (X,Y) of
-    (INL vX,INL vY) => encode_element2d_vv bnd R vX vY Tss
-  | (INL vX,INR cY) => encode_element2d_vc bnd R vX cY Tss
-  | (INR cX,INL vY) => encode_element2d_cv bnd R cX vY Tss
-  | (INR cX,INR cY) => encode_element2d_cc bnd R cX cY Tss
 End
 
 (* The top-level encodings *)
